some lemmas, and coset

Math/Algebra/C2_Groups/C2_1_Basics/definitions.lean
@@ -173,3 +173,12 @@ Coe (idGroupMorphism G) (GroupHomomorphism G G) := {
 -- two groups are called isomorphic, iff there exists a group-isomorphism between the two groups
 def groupsAreIsomorphic (G1 : Type u) (G2 : Type v) [MyGroup G1] [MyGroup G2] : Prop :=
   ∃ _ : GroupIsomorphism G1 G2, true
+
+
+-- left coset = linke Nebenklasse
+def left_coset (G : Type u) [MyGroup G] (H : Subgroup G) (g : G) : Set G :=
+  { x | ∃ h : H.carrier, x = MyGroup.mul g ↑h }
+
+-- right coset = rechte Nebenklasse
+def right_coset (G : Type u) [MyGroup G] (H : Subgroup G) (g : G) : Set G :=
+  { x | ∃ h : H.carrier, x = MyGroup.mul ↑h g }
